examples/store/proofs/server.v
@@ -166,10 +166,7 @@ wp_pures.
 wp_apply (RPC.wp_confirm (db_server_ready skA (ss_key ss) db)
            with "[] [] [] [$ready]") => //.
 { do 3!iSplit => //. }
-iIntros "%cs (conn & ready)".
-iPoseProof (RPC.server_public_compromised with "conn ready")
-  as "[conn >ready]".
-wp_pures.
+iIntros "%cs (conn & ready)". wp_pures.
 iApply (wp_fork with "[conn vdb locked ready]").
 { iModIntro.
   wp_apply (wp_server_conn_handler
